Added functions to the bignum library

examples/stateful_bignum/carry_st.fsi
@@ -1,0 +1,46 @@
+(* STATUS : lax type checks but not verified, work in progress *)
+
+module Carry
+
+open Heap 
+open ST
+open Limb
+open Bigint
+open IntLib
+open Seq
+open Axiomatic
+open Eval
+open Array
+
+val blit : #a:Type -> i:array a -> i_dix:nat -> o:array a -> o_idx:nat -> len:nat -> 
+		  ST unit
+		     (requires (fun h -> 
+				(contains h i)
+				/\ (contains h o)
+				/\ (len + i_idx <= Seq.length (sel h i))
+				/\ (len + o_idx <= Seq.length (sel h o))
+				   (* Need of a separation clause ? *)
+		     (ensures (fun h0 u h1 -> 
+			       (contains h1 i)
+			       /\ (contains h1 o)
+			       /\ (modifies !{o} h0 h1)
+			       /\ (len + i_idx <= Seq.length (sel h0 i))
+			       /\ (len + o_idx <= Seq.length (sel h0 o))
+			       /\ (forall (n:nat). n < len 
+				   ==> Seq.index (sel h1 o) (n+o_idx) = Seq.index (sel h0 i) (n+i_idx))
+		     ))
+
+val carry : 
+  a:bigint -> 
+  ST unit
+     (requires (fun h -> 
+		(contains h a)
+     ))
+     (ensures (fun h0 u h1 ->
+	       (contains h0 a)
+	       /\ (contains h1 a)
+	       /\ (modifies !{Bigint63.data a} h0 h1)
+	       /\ (Normalized h1 a)
+	       /\ (eval h1 a (getLength h1 a) = eval h0 a (getLength h0 a))
+     ))
+	       
