examples/stateful_bignum/retemplate_st.fsi
@@ -1,0 +1,22 @@
+module Retemplate 
+
+open Heap
+open ST
+open Bigint
+
+val retemplate:
+  a:bigint -> t:template ->
+  ST bigint
+     (requires (fun h ->
+		(inHeap h a)
+		/\ (Normalized h a)
+     ))
+     (ensures (fun h0 b h1 ->
+	       (inHeap h1 b)
+	       /\ (inHeap h0 a)
+	       /\ (Normalized h0 a)
+	       /\ (modifies !{} h0 h1)
+	       /\ not(contains h0 (Bigint63.data b))
+	       /\ (Bigint63.t b = t)
+	       /\ (eval h1 b (getLength h1 b) = eval h0 a (getLength h0 a))
+     ))
